still stuck at composition lemma

subst.fst
@@ -7,48 +7,51 @@ type subst = list (variable * term)
 val isnt_cyclic : subst -> Tot bool
 val get_Images : subst -> Tot (list term)
 val get_Domain : subst -> Tot (list variable)
-val check_presence_varlist_termlist : list variable -> list term -> Tot bool
+val check_presence_vars_in_terms : list variable -> list term -> Tot bool
 
 val mem: #a:eqtype -> a -> list a -> Tot bool
-let rec mem #a x xs =
-  match xs with
+let rec mem #a x xs = match xs with
   | [] -> false
   | hd::tl -> hd=x || mem x tl
 
-let rec get_Images st =
-match st with
-| [] -> []
-| hd::tl -> (snd hd)::(get_Images tl)
+let rec get_Images st = match st with
+  | [] -> []
+  | hd::tl -> (snd hd)::(get_Images tl)
 
-let rec get_Domain st =
-match st with
-| [] -> []
-| hd::tl -> (fst hd)::(get_Domain tl)
+let rec get_Domain st = match st with
+  | [] -> []
+  | hd::tl -> (fst hd)::(get_Domain tl)
 
-let rec check_presence_varlist_termlist lv lt =
-  match lv with
+let rec check_presence_vars_in_terms lv lt = match lv with
   | [] -> true
-  | hd::tl -> (is_var_present_list hd lt) && (check_presence_varlist_termlist tl lt)
+  | hd::tl -> (is_var_present_list hd lt) && (check_presence_vars_in_terms tl lt)
+
+val aux_lemma1 : lv:list variable -> hd:term -> tl:list term -> Lemma
+  (requires true)
+  (ensures (check_presence_vars_in_terms lv (hd::tl)) ==> (check_presence_vars_in_terms lv tl) )
+let rec aux_lemma1 lv hd tl = match lv with
+  | [] -> ()
+  | first::last -> aux_lemma1 last hd tl
 
 let isnt_cyclic st =
   let lv = get_Domain st in
   let lt = get_Images st in
-  check_presence_varlist_termlist lv lt
+  check_presence_vars_in_terms lv lt
 
+val aux_lemma2 : hd:(variable*term) -> tl:subst -> Lemma
+  (requires true)
+  (ensures isnt_cyclic (hd::tl) ==> isnt_cyclic tl )
+let aux_lemma2 hd tl = aux_lemma1 (get_Domain tl) (snd hd) (get_Images tl)
 
 val apply : subst -> term ->Tot term
 val apply_list : subst -> l1:list term ->Tot (l2:list term{FStar.List.Tot.length l1 = FStar.List.Tot.length l2})
 
-val get_Term : variable -> subst -> Tot term
+val get_Term : v:variable -> s:subst{ mem v (get_Domain s) } -> Tot term
 
-
-(** bad function rewrite later**)
 let rec get_Term v st= match st with
-| hd::tl -> if (fst hd)=v then (snd hd) else (get_Term v tl)
-| [] -> Var v
+  | hd::tl -> if (fst hd)=v then (snd hd) else (get_Term v tl)
 
-let rec apply st t =
-  match t with
+let rec apply st t = match t with
   | Var v -> if mem v (get_Domain st) then (get_Term v st) else t
   | Func s args -> Func s (apply_list st args)
   | Name n -> t
@@ -58,8 +61,7 @@ let rec apply st t =
 
 val distinct_lists : #a:eqtype -> list a -> list a -> Tot bool
 
-let rec distinct_lists #a l1 l2 =
-match l1 with
+let rec distinct_lists #a l1 l2 = match l1 with
   | [] -> true
   | hd::tl -> not(mem hd l2) && (distinct_lists tl l2)
 
@@ -72,11 +74,21 @@ let distinct_domain st1 st2 =
 
 val is_composable : subst -> subst -> Tot bool
 
-let is_composable st1 st2 = (distinct_domain st1 st2 ) && (isnt_cyclic (FStar.List.Tot.append st1 st2) )
+let is_composable st1 st2 = (distinct_domain st1 st2)
+                            && isnt_cyclic st1 && isnt_cyclic st2
+                            && check_presence_vars_in_terms (get_Domain st1) (get_Images st2)
+
+val aux_lemma3 : hd:(variable*term) -> tl:subst -> st:subst -> Lemma
+  (requires is_composable (hd::tl) st)
+  (ensures is_composable tl st)
+
+let rec aux_lemma3 hd tl st = aux_lemma2 hd tl
 
 val compose : st1:subst -> st2:subst -> Tot subst
 
-let rec compose st1 st2 = FStar.List.Tot.append st1 st2
+let rec compose st1 st2 = match st1 with
+ | [] -> st2
+ | hd::tl -> (fst hd,apply st2 (snd hd))::(compose tl st2)
 
 (*
 val is_unify : term -> term -> bool
@@ -85,25 +97,66 @@ val mgs : t1:term -> t2:term{ is_unify t1 t2 } -> subst*)
 
 
 val ground_term_lemma : st:subst -> t:term -> Lemma (requires (is_ground t)) (ensures (apply st t)=t)
-val ground_list_term_lemma : st:subst -> lt:list term -> Lemma (requires (is_ground_list lt)) (ensures (apply_list st lt)=lt)
+val ground_list_term_lemma : st:subst -> lt:list term -> Lemma
+  (requires (is_ground_list lt))
+  (ensures (apply_list st lt)=lt)
 
-let rec ground_term_lemma st t =
-  match t with
+let rec ground_term_lemma st t = match t with
   | Func _ args -> ground_list_term_lemma st args
   | Name _ -> ()
-  and ground_list_term_lemma st lt =
-  match lt with
+  and ground_list_term_lemma st lt = match lt with
   | [] -> ()
   | hd::tl -> (ground_term_lemma st hd) ; (ground_list_term_lemma st tl)
 
-val compose_lemma : st1:subst -> st2:subst-> Lemma (requires (is_composable st1 st2)) (ensures forall (x:variable). mem x (get_Domain (compose st1 st2)) <==> ( (mem x (get_Domain st1) || mem x (get_Domain st2)) && not( mem x (get_Domain st1) && mem x (get_Domain st2))))
+val compose_aux_lemma1 : st1:subst -> st2:subst -> Lemma
+  (requires (is_composable st1 st2))
+  (ensures forall (x:variable).
+  mem x (get_Domain (compose st1 st2)) <==>
+    ((mem x (get_Domain st1) || mem x (get_Domain st2))
+      && not(mem x (get_Domain st1) && mem x (get_Domain st2)) )
+  )
 
-let rec compose_lemma st1 st2 =
-  match st1 with
+let rec compose_aux_lemma1 st1 st2 = match st1 with
   | [] -> ()
-  | hd::tl -> compose_lemma tl st2
+  | hd::tl -> aux_lemma3 hd tl st2 ; compose_aux_lemma1 tl st2
 
-(*val assoc_lemma : st1:subst -> st2:subst -> t:term -> Lemma (requires is_composable st1 st2)(ensures apply (compose st1 st2) t= apply st2 (apply st1 t))
-let rec assoc_lemma st1 st2 t=
-  match t with
-  | Var v ->*)
+val compose_aux_lemma2a : x:variable -> st1:subst -> st2:subst -> Lemma
+  (requires is_composable st1 st2)
+  (ensures (  (mem x (get_Domain st1)) ==> (mem x (get_Domain (compose st1 st2))) ) )
+
+val compose_aux_lemma2b : x:variable -> st1:subst -> st2:subst -> Lemma
+  (requires is_composable st1 st2)
+  (ensures (  (mem x (get_Domain st2)) ==> (mem x (get_Domain (compose st1 st2))) ) )
+
+let rec compose_aux_lemma2a x st1 st2 = match st1 with
+  | [] -> ()
+  | hd::tl -> aux_lemma3 hd tl st2 ; compose_aux_lemma2a x tl st2
+
+let rec compose_aux_lemma2b x st1 st2 = match st1 with
+  | [] -> ()
+  | hd::tl -> aux_lemma3 hd tl st2 ; compose_aux_lemma2b x tl st2
+
+val compose_aux_lemma3 : st1:subst -> st2:subst -> x:variable -> Lemma
+ (requires (is_composable st1 st2))
+ (ensures ( (mem x (get_Domain st1) ==> (get_Term x (compose st1 st2) = apply st2 (get_Term x st1))) /\
+            (mem x (get_Domain st2) ==> (get_Term x (compose st1 st2) = get_Term x st2)) ) )
+
+let rec compose_aux_lemma3 st1 st2 x = match st1 with
+  | [] -> ()
+  | hd::tl -> if x=fst hd then () else aux_lemma3 hd tl st2 ; compose_aux_lemma1 st1 st2;  compose_aux_lemma3 tl st2 x
+
+(*val compose_lemma : st1:subst -> st2:subst -> t:term -> Lemma
+  (requires is_composable st1 st2)
+  (ensures apply (compose st1 st2) t= apply st2 (apply st1 t))
+
+val compose_list_lemma : st1:subst -> st2:subst -> lt:list term -> Lemma
+  (requires is_composable st1 st2)
+  (ensures apply_list (compose st1 st2) lt = apply_list st2 (apply_list st1 lt))
+
+let rec compose_lemma st1 st2 t = match t with
+  | Var v -> compose_aux_lemma3 st1 st2 v
+  | Name n -> ()
+  | Func s args -> compose_list_lemma st1 st2 args
+  and compose_list_lemma st1 st2 lt = match lt with
+  | [] -> ()
+  | hd::tl -> compose_lemma st1 st2 hd ; compose_list_lemma st1 st2 tl*)
